Proof - ordering conflicting ops

ew.fst
@@ -1,319 +1,279 @@
 module Ew
+
 open FStar.List.Tot
 
-#set-options "--query_stats"
+val get_id : #op:eqtype -> (nat * op) -> nat
+let get_id (id, _) = id
 
-open Library
+val get_op : #op:eqtype -> (nat * op) -> op
+let get_op (_, op) = op
 
-type s = nat * bool
+val mem_id : #op:eqtype
+           -> id:nat
+           -> l:list (nat * op)
+           -> Tot (b:bool{(exists op. mem (id,op) l) <==> b=true})
+let rec mem_id n l =
+  match l with
+  |[] -> false
+  |(id,_)::xs -> (n = id) || mem_id n xs
 
-type rval = |Val : bool -> rval
-            |Bot
+val unique_id : #op:eqtype 
+              -> l:list (nat * op)
+              -> Tot bool
+let rec unique_id l =
+  match l with
+  |[] -> true
+  |(id,_)::xs -> not (mem_id id xs) && unique_id xs
 
-type op = 
+val get_eve : #op:eqtype 
+            -> id:nat 
+            -> l:list (nat * op){unique_id l /\ mem_id id l}
+            -> Tot (s:(nat * op) {get_id s = id /\ mem s l})
+let rec get_eve id l =
+  match l with
+  |(id1, x)::xs -> if id = id1 then (id1, x) else get_eve id xs 
+
+val forallb : #a:eqtype
+            -> f:(a -> bool)
+            -> l:list a
+            -> Tot (b:bool{(forall e. mem e l ==> f e) <==> b = true})
+let rec forallb #a f l = 
+  match l with
+  |[] -> true
+  |hd::tl -> if f hd then forallb f tl else false
+
+val existsb : #a:eqtype
+            -> f:(a -> bool)
+            -> l:list a 
+            -> Tot (b:bool{(exists e. mem e l /\ f e) <==> b = true})
+let rec existsb #a f l =
+  match l with
+  |[] -> false
+  |hd::tl -> if f hd then true else existsb f tl
+
+val sorted : #op:eqtype
+           -> l:list(nat * op){unique_id l} -> bool
+let rec sorted #op l =
+  match l with
+  |[] -> true
+  |x::[] -> true
+  |x::xs -> forallb (fun (e:(nat * op)) -> fst x < fst e) xs && sorted xs
+
+val filter : #a:eqtype
+           -> f:(a -> bool)
+           -> l:list a
+           -> Tot (l1:list a {forall e. mem e l1 <==> mem e l /\ f e})
+let rec filter #a f l = 
+  match l with
+  |[] -> []
+  |hd::tl -> if f hd then hd::(filter f tl) else filter f tl
+
+/////////////////////////////////////////
+
+type op =
   |Enable
   |Disable
-  |Rd
 
-val init : nat * bool
-let init = (0, false)
+///SEQUENTIAL DATA TYPE IMPLEMENTATION///
 
-let pre_cond_do s1 op = true
-let pre_cond_prop_do tr s1 op = true
+type s = bool
 
-val do : s1:s -> o:(nat * op) -> Tot (s2:(s * rval) {(get_op o = Enable ==> s2 = ((fst s1 + 1, true), Bot)) /\
-                                                 (get_op o = Disable ==> s2 = ((fst s1, false), Bot)) /\
-                                                 (get_op o = Rd ==> s2 = (s1, Val (snd s1)))})
-let do (c,f) e = 
-  match e with
-  |(_,Enable) -> ((c + 1, true), Bot)
-  |(_,Disable) -> ((c, false), Bot)
-  |(_,Rd) -> ((c,f), Val f)
+let init = false
 
-val sum : l:(list (nat * op))
-        -> Tot (n:nat {n = (List.Tot.length (filter (fun a -> get_op a = Enable) l))}) (decreases %[l])
-let rec sum l =
+val do : s -> (nat * op) -> s
+let do s op =
+  match op with
+  |(_,Enable) -> true
+  |(_,Disable) -> false
+
+val spec : s1:s -> o1:(nat * op) -> o2:(nat * op) -> s
+let spec s1 o1 o2 =
+  match get_op o1, get_op o2 with
+  |Enable, Disable -> do (do s1 o2) o1
+  |_ -> do (do s1 o1) o2
+
+val fold : st:s -> l:list (nat * op){unique_id l} -> Tot s (decreases l)
+let rec fold s l =
   match l with
-  |[] -> 0
-  |(_, Enable)::xs -> sum xs + 1
-  |_::xs -> sum xs
+  |[] -> s
+  |x::xs -> fold (do s x) xs
 
-val flag : tr:ae op
-         -> Tot (b:bool {(b = true) <==> (exists e. (mem e tr.l /\ get_op e = Enable /\ 
-                   (forall d. (mem d tr.l /\ get_id e <> get_id d /\ get_op d = Disable) ==> not (tr.vis e d))))})
+////////////MRDT IMPLEMENTATION////////////
 
-let flag tr = 
-  existsb (fun e -> (forallb (fun d -> not (tr.vis e d)) 
-                 (filter (fun d -> get_op d = Disable && get_id e <> get_id d) tr.l))) 
-          (filter (fun e -> get_op e = Enable) tr.l)
+type s' = nat * bool
 
-val spec : o:(nat * op) -> tr:ae op -> rval
-let spec o tr = 
-  match o with
-  |(_,Enable) -> Bot
-  |(_,Disable) -> Bot
-  |(_,Rd) -> Val (flag tr)
+val init' : s'
+let init' = (0, false)
 
-val sim : tr:ae op
-        -> s1:s
-        -> Tot (b:bool {b = true <==> ((fst s1 = sum tr.l) /\ (snd s1 = flag tr))})
-let sim tr s1 = (s1 = (sum tr.l, flag tr))
+let pre_cond_do' s o = true
 
-val lemma11 : l:list(nat * op) {unique_id l}
-            -> a:list(nat * op) {unique_id a}
-            -> Lemma (requires (forall e. mem e l ==> not (mem_id (get_id e) a)))
-                    (ensures (sum (union1 l a) = sum l + sum a))
-let rec lemma11 l a =
-  match l,a with
-  |[],[] -> ()
-  |x::xs,_ -> lemma11 xs a
-  |[],_ -> ()
+val do' : st:s' -> o:(nat * op) -> st1:s'{(get_op o = Enable <==> (st1 = (fst st + 1, true))) /\
+                                      (get_op o = Disable <==> (st1 = (fst st, false)))}
+let do' s' op =
+  match op with
+  |(_,Enable) -> (fst s' + 1, true)
+  |(_,Disable) -> (fst s', false)
 
-val lemma1 : l:ae op
-           -> a:ae op
-           -> Lemma (requires (forall e. mem e l.l ==> not (mem_id (get_id e) a.l)))
-                   (ensures (forall e. mem e (union l a).l <==> mem e l.l \/ mem e a.l) /\
-                            (sum (union l a).l = sum l.l + sum a.l))
-let lemma1 l a = lemma11 l.l a.l
+val tl : l:list(nat * op){l <> []} -> Tot (t:(nat * op){mem t l})
+let rec tl l =
+  match l with
+  |[x] -> x
+  |x::xs -> tl xs
 
-val merge_flag : l:s 
-               -> a:s{fst a >= fst l}
-               -> b:s{fst b >= fst l}
+val fold' : st:s' -> l:list (nat * op)
+          -> Pure s'
+            (requires unique_id l)
+            (ensures (fun r -> ((l <> [] /\ (forall e. mem e l ==> get_op e <> Disable)) ==> (fst r > fst st)) /\
+                             (fst r >= fst st) /\ (l <> [] /\ get_op (tl l) = Enable ==> (fst r > fst st)) /\
+                             (l = [] ==> r = st) /\
+                             ((snd r = true) <==> ((l = [] /\ snd st = true) \/ (l <> [] /\ get_op (tl l) = Enable))) /\
+                             (l <> [] /\ get_op (tl l) = Disable ==> snd r = false)))
+              (decreases l)
+let rec fold' s l =
+  match l with
+  |[] -> s
+  |x::xs -> fold' (do' s x) xs
+
+val pre_cond_merge' : l:s' -> a:s' -> b:s' -> bool
+let pre_cond_merge' l a b = fst a >= fst l && fst b >= fst l
+
+val merge_flag : l:s'
+               -> a:s'{fst a >= fst l}
+               -> b:s'{fst b >= fst l}
                -> Tot (b1:bool {(b1 = true <==> (snd a = true /\ snd b = true) \/ 
                                              (snd a = true /\ snd b = false /\ fst a > fst l) \/
                                              (snd b = true /\ snd a = false /\ fst b > fst l)) /\
-                               (b1 = false <==> (snd a = false /\ snd b = false) \/ 
-                                              (snd a = true /\ snd b = false /\ fst a = fst l) \/
-                                              (snd b = true /\ snd a = false /\ fst b = fst l))}) 
+                                (b1 = false <==> (snd a = false /\ snd b = false) \/ 
+                                               (snd a = true /\ snd b = false /\ fst a = fst l) \/
+                                               (snd b = true /\ snd a = false /\ fst b = fst l))})
 let merge_flag l a b =
   let lc = fst l in
   let ac = fst a in
   let bc = fst b in
   let af = snd a in
   let bf = snd b in
-  if af && bf then true
-    else if not af && not bf then false
-      else if af then ac - lc > 0
-        else bc - lc > 0
+    if af && bf then true
+      else if not af && not bf then false
+        else if af then ac - lc > 0
+          else bc - lc > 0
 
-val pre_cond_merge : s -> s -> s -> bool
-let pre_cond_merge l a b = fst a >= fst l && fst b >= fst l
-
-let pre_cond_prop_merge ltr l atr a btr b = true
-
-val merge : l:s
-          -> a:s
-          -> b:s
-          -> Pure s
-            (requires pre_cond_merge l a b)
-            (ensures (fun res -> (snd res = true <==> (snd a = true /\ snd b = true) \/ 
-                                                 (snd a = true /\ snd b = false /\ fst a > fst l) \/
-                                                 (snd b = true /\ snd a = false /\ fst b > fst l)) /\
-                              (snd res = false <==> (snd a = false /\ snd b = false) \/
-                                                  (snd a = true /\ snd b = false /\ fst a = fst l) \/ 
-                                                  (snd b = true /\ snd a = false /\ fst b = fst l)) /\
-                              (fst res = fst a + fst b - fst l)))
-let merge l a b =
+val merge' : l:s' 
+           -> a:s'
+           -> b:s'
+           -> Pure s'
+             (requires pre_cond_merge' l a b)
+             (ensures (fun r -> r = (fst a + fst b - fst l, merge_flag l a b)))
+let merge' l a b =
   let c = fst a + fst b - fst l in
   let f = merge_flag l a b in
   c, f
 
-val lemma21 : l:list(nat * op) {unique_id l}
-            -> a:list(nat * op) {unique_id a}
-            -> b:list(nat * op) {unique_id b}
-            -> Lemma (requires (forall e. mem e l ==> not (mem_id (get_id e) a)) /\
-                              (forall e. mem e a ==> not (mem_id (get_id e) b)) /\
-                              (forall e. mem e l ==> not (mem_id (get_id e) b)))
-                    (ensures (forall e. mem e (abs_merge1 l a b) <==> mem e l \/ mem e a \/ mem e b) /\
-                             (sum (abs_merge1 l a b) = sum a + sum b + sum l))
-                             (decreases %[l;a;b])
-#set-options "--z3rlimit 1000"
-let rec lemma21 l a b =
-  match l,a,b with
-  |[],[],[] -> ()
-  |x::xs,_,_ -> lemma21 xs a b
-  |[],x::xs,_ -> lemma21 [] xs b
-  |[],[],_ -> ()
+////////////////////////////////////////////
 
-val lemma2 : l:ae op
-           -> a:ae op
-           -> b:ae op
-           -> Lemma (requires (forall e. mem e l.l ==> not (mem_id (get_id e) a.l)) /\
-                             (forall e. mem e a.l ==> not (mem_id (get_id e) b.l)) /\
-                             (forall e. mem e l.l ==> not (mem_id (get_id e) b.l)))
-                   (ensures (forall e. mem e (abs_merge l a b).l <==> mem e l.l \/ mem e a.l \/ mem e b.l) /\
-                            (sum (abs_merge l a b).l = sum a.l + sum b.l + sum l.l))
-let lemma2 l a b = lemma21 l.l a.l b.l
+val eq : st:s -> st':s' -> bool
+let eq s s' = s = snd s'
 
-val lem_sum : l:list (nat * op)
-            -> Lemma (requires (unique_id l))
-                    (ensures (sum l > 0 <==> (exists e. mem e l /\ get_op e = Enable)) /\
-                             (sum l = 0 <==> ((forall e. mem e l ==> 
-                                    (get_op e = Disable \/ get_op e = Rd) /\ l <> []) \/ l = [])))
-                             (decreases l)
-let rec lem_sum l = 
-  match l with
-  |[] -> ()
-  |x::xs -> lem_sum xs
+val eq_m : a:s' -> b:s' -> bool
+let eq_m a b = snd a = snd b
 
-val prop_merge : ltr:ae op
-               -> l:s
-               -> atr:ae op
-               -> a:s
-               -> btr:ae op
-               -> b:s
-               -> Lemma (requires (forall e. mem e ltr.l ==> not (mem_id (get_id e) atr.l)) /\
-                                 (forall e. mem e atr.l ==> not (mem_id (get_id e) btr.l)) /\
-                                 (forall e. mem e ltr.l ==> not (mem_id (get_id e) btr.l)) /\
-                                 (sim ltr l /\ sim (union ltr atr) a /\ sim (union ltr btr) b))
-                       (ensures (pre_cond_merge l a b) /\ (sim (abs_merge ltr atr btr) (merge l a b)))
+val prop_init : unit -> Lemma (ensures (eq init init'))
+let prop_init () = ()
 
-#set-options "--z3rlimit 100000"
-let prop_merge ltr l atr a btr b = 
-  lemma1 ltr atr;
-  lemma1 ltr btr;
-  lemma2 ltr atr btr;
-  lem_sum atr.l;
-  lem_sum btr.l
+val prop_equivalence : a:s' -> b:s' -> o:(nat * op)
+                     -> Lemma (requires (eq_m a b /\ pre_cond_do' a o /\ pre_cond_do' b o))
+                             (ensures (eq_m (do' a o) (do' b o)))
+let prop_equivalence a b o = ()
 
-val prop_do : tr:ae op
-            -> st:s
-            -> op:(nat * op)
-            -> Lemma (requires (sim tr st) /\ (not (mem_id (get_id op) tr.l)) /\
-                              (forall e. mem e tr.l ==> get_id e < get_id op) /\ get_id op > 0)
-                    (ensures (sim (abs_do tr op) (get_st (do st op))))
-let prop_do tr st op = ()
+val prop_do : st:s -> st':s' -> o:(nat * op)
+            -> Lemma (requires (eq st st'))
+                    (ensures (eq (do st o) (do' st' o)))
+let prop_do s s' op = ()
 
-val convergence : tr:ae op
-                 -> a:s
-                 -> b:s
-                 -> Lemma (requires (sim tr a /\ sim tr b))
-                         (ensures a = b)
-let convergence tr a b = ()
+val inverse : st:s' -> o:(nat * op) 
+            -> Pure (list s') 
+              (requires (get_op o = Enable ==> fst st > 0) /\
+                        (get_op o = Disable <==> snd st = false))
+              (ensures (fun r -> (forall e. mem e r ==> st = do' e o)))
+let inverse a o =
+  match o with
+  |(_, Enable) -> [(fst a - 1, true); (fst a - 1, false)]
+  |(_, Disable) -> [(fst a, false); (fst a, true)]
 
-val prop_spec : tr:ae op
-              -> st:s
-              -> op:(nat * op)
-              -> Lemma (requires (sim tr st) /\ (not (mem_id (get_id op) tr.l)) /\
-                                (forall e. mem e tr.l ==> get_id e < get_id op) /\ get_id op > 0)
-                      (ensures (get_rval (do st op) = spec op tr))
-let prop_spec tr st op = ()
+val append : l1:list(nat * op) -> l2:list(nat * op)
+           -> Pure (list (nat * op))
+                  (requires (forall e. mem e l1 ==> not (mem_id (get_id e) l2)) /\
+                            unique_id l1 /\ unique_id l2)
+                  (ensures (fun r -> (forall e. mem e r <==> mem e l1 \/ mem e l2) /\ unique_id r /\
+                                  (l2 <> [] ==> tl r = tl l2)))
+                  (decreases %[l1;l2])
+let rec append l1 l2 =
+  match l1, l2 with
+  |[],[] -> []
+  |x::xs,_ -> x::(append xs l2)
+  |[],x::xs -> x::(append [] xs)
 
-instance ew : mrdt s op rval = {
-  Library.init = init;
-  Library.spec = spec;
-  Library.sim = sim;
-  Library.pre_cond_do = pre_cond_do;
-  Library.pre_cond_prop_do = pre_cond_prop_do;
-  Library.pre_cond_merge = pre_cond_merge;
-  Library.pre_cond_prop_merge = pre_cond_prop_merge;
-  Library.do = do;
-  Library.merge = merge;
-  Library.prop_do = prop_do;
-  Library.prop_merge = prop_merge;
-  Library.prop_spec = prop_spec;
-  Library.convergence = convergence
-}
+val prop_merge1 : l:s' -> a:s' -> b:s' 
+                -> atr:list(nat * op) -> o1:(nat * op) 
+                -> btr:list(nat * op) -> o2:(nat * op) 
+                -> Lemma (requires (unique_id atr /\ unique_id btr /\ get_id o1 <> get_id o2 /\
+                                  (forall e. mem e atr ==> not (mem_id (get_id e) btr)) /\
+                                  not (mem_id (get_id o1) atr) /\ not (mem_id (get_id o1) btr) /\
+                                  not (mem_id (get_id o2) atr) /\ not (mem_id (get_id o2) btr) /\
+                                  a = fold' l (append atr [o1]) /\ b = fold' l (append btr [o2])))
+                        (ensures (forall ia ib. mem ia (inverse a o1) /\ mem ib (inverse b o2) ==>
+                                   (let merge_prefix = (merge' l ia ib) in 
+                                      ((merge' l a b) = (merge' merge_prefix (do' merge_prefix o1) (do' merge_prefix o2))))))
+let prop_merge1 l a b atr o1 btr o2 = ()
+
+val prop_merge2 : l:s' -> a:s' -> b:s' -> op1:(nat * op) -> op2:(nat * op)
+                -> Lemma (requires (a = do' l op1 /\ b = do' l op2 /\ get_id op1 <> get_id op2))
+                        (ensures (pre_cond_merge' l a b) /\
+                                 (forall sl. eq sl l ==> (eq (spec sl op1 op2) (merge' l a b))))
+let prop_merge2 l a b opa opb = ()
+
+(*)val prop_merge3 : l:s' -> a:s' -> atr:list(nat * op) -> o1:(nat * op)
+                -> Lemma (requires (unique_id atr /\ not (mem_id (get_id o1) atr) /\
+                                  (a = fold' l (append atr [o1])) /\
+                                  (forall e. mem e (inverse a o1) ==> e = fold' l atr)))
+                        (ensures (forall ia. mem ia (inverse a o1) ==>
+                                    (merge' l a l) = (merge' l ia (do' l o1))))
+let prop_merge3 l a atr o1 = ()*)
+
+val prop_merge4 : l:s' -> a:s' -> op1:(nat * op)
+                -> Lemma (requires (a = do' l op1))
+                        (ensures (pre_cond_merge' l a l) /\
+                                 (forall sl. eq sl l ==> (eq (do sl op1) (merge' l a l))))
+let prop_merge4 l a op1 = ()
+
+val idempotence : a:s'
+                -> Lemma (ensures (a = (merge' a a a)))
+let idempotence a = ()
+
+val commutativity : l:s' 
+                  -> a:s'
+                  -> b:s'
+                  -> Lemma (requires (exists atr btr. unique_id atr /\ unique_id btr /\ a = fold' l atr /\ b = fold' l btr))
+                          (ensures (merge' l b a = merge' l a b))
+let commutativity l a b = ()
+
+val associativity : l:s'
+                  -> a:s'
+                  -> b:s'
+                  -> c:s'
+                  -> Lemma (requires (exists atr btr ctr. unique_id atr /\ unique_id btr /\ unique_id ctr /\
+                                     a = fold' l atr /\ b = fold' l btr /\ c = fold' l ctr))
+                          (ensures (merge' l a (merge' l b c) = merge' l (merge' l a b) c))
+let associativity l a b c = ()
 
 
-(* Additional lemmas for prop_merge  
+val prop_merge00 : l:s' -> a:s' -> b:s' -> op1:(nat * op) -> op2:(nat * op)
+                 -> Lemma (requires (a = do' l op1 /\ b = do' l op2 /\ get_id op1 <> get_id op2 /\
+                                    (exists atr btr. unique_id atr /\ unique_id btr /\
+                                    a = fold' l atr /\ b = fold' l btr)))
+                         (ensures (pre_cond_merge' l a b) /\
+                                  (forall sl. eq sl (merge' l a b) ==> 
+                                     (eq (spec sl op1 op2) (merge' (merge' l a b)
+                                                                   (do' (merge' l a b) op1) 
+                                                                   (do' (merge' l a b) op2)))))
 
-val prop_merge1 : ltr:ae op
-                -> l:s
-                -> atr:ae op
-                -> a:s
-                -> btr:ae op
-                -> b:s
-                -> Lemma (requires (forall e. mem e ltr.l ==> not (mem_id (get_id e) atr.l)) /\
-                                  (forall e. mem e atr.l ==> not (mem_id (get_id e) btr.l)) /\
-                                  (forall e. mem e ltr.l ==> not (mem_id (get_id e) btr.l)) /\
-                                  (sim ltr l /\ sim (union ltr atr) a /\ sim (union ltr btr) b) /\
-                                  (pre_cond_merge l a b))
-                        (ensures ((snd a = true /\ snd b = true) ==> flag (abs_merge ltr atr btr) = true) /\
-                                 ((snd a = false /\ snd b = false) ==> flag (abs_merge ltr atr btr) = false))
-let prop_merge1 ltr l atr a btr b = ()
-
-val prop_merge2 : ltr:ae op
-                -> l:s
-                -> atr:ae op
-                -> a:s
-                -> btr:ae op
-                -> b:s
-                -> Lemma (requires (forall e. mem e ltr.l ==> not (mem_id (get_id e) atr.l)) /\
-                                  (forall e. mem e atr.l ==> not (mem_id (get_id e) btr.l)) /\
-                                  (forall e. mem e ltr.l ==> not (mem_id (get_id e) btr.l)) /\
-                                  (sim ltr l /\ sim (union ltr atr) a /\ sim (union ltr btr) b) /\
-                                  (pre_cond_merge l a b))
-                        (ensures ((snd a = true /\ snd b = false /\ fst a = fst l) ==> 
-                                       flag (abs_merge ltr atr btr) = false) /\
-                                 ((snd b = true /\ snd a = false /\ fst b = fst l) ==> 
-                                       flag (abs_merge ltr atr btr) = false))
-
-#set-options "--z3rlimit 10000"
-let prop_merge2 ltr l atr a btr b = 
-  lemma1 ltr atr; lemma1 ltr btr;
-  lem_sum atr.l; lem_sum btr.l
-
-val prop_merge3 : ltr:ae op
-                -> l:s
-                -> atr:ae op
-                -> a:s
-                -> btr:ae op
-                -> b:s
-                -> Lemma (requires (forall e. mem e ltr.l ==> not (mem_id (get_id e) atr.l)) /\
-                                  (forall e. mem e atr.l ==> not (mem_id (get_id e) btr.l)) /\
-                                  (forall e. mem e ltr.l ==> not (mem_id (get_id e) btr.l)) /\
-                                  (sim ltr l /\ sim (union ltr atr) a /\ sim (union ltr btr) b) /\
-                                  (pre_cond_merge l a b))
-                        (ensures ((snd a = true /\ snd b = false /\ fst a > fst l) ==> 
-                                       flag (abs_merge ltr atr btr) = true) /\
-                                 ((snd b = true /\ snd a = false /\ fst b > fst l) ==> 
-                                       flag (abs_merge ltr atr btr) = true))
-
-#set-options "--z3rlimit 10000"
-let prop_merge3 ltr l atr a btr b = 
-  lemma1 ltr atr; lemma1 ltr btr;
-  lemma2 ltr atr btr; 
-  lem_sum atr.l; lem_sum btr.l
-
-val prop_merge4 : ltr:ae op
-                -> l:s 
-                -> atr:ae op
-                -> a:s 
-                -> btr:ae op
-                -> b:s 
-                -> Lemma (requires (forall e. mem e ltr.l ==> not (mem_id (get_id e) atr.l)) /\
-                                  (forall e. mem e atr.l ==> not (mem_id (get_id e) btr.l)) /\
-                                  (forall e. mem e ltr.l ==> not (mem_id (get_id e) btr.l)) /\
-                                  (sim ltr l /\ sim (union ltr atr) a /\ sim (union ltr btr) b) /\
-                                  (pre_cond_merge l a b))
-                        (ensures (sum (abs_merge ltr atr btr).l = fst (merge l a b)))
-
-#set-options "--z3rlimit 1000"
-let prop_merge4 ltr l atr a btr b = 
-  lemma1 ltr atr; 
-  lemma1 ltr btr;
-  lemma2 ltr atr btr; ()
-
-val prop_merge5 : ltr:ae op
-                -> l:s
-                -> atr:ae op
-                -> a:s
-                -> btr:ae op
-                -> b:s
-                -> Lemma (requires (forall e. mem e ltr.l ==> not (mem_id (get_id e) atr.l)) /\
-                                  (forall e. mem e atr.l ==> not (mem_id (get_id e) btr.l)) /\
-                                  (forall e. mem e ltr.l ==> not (mem_id (get_id e) btr.l)) /\
-                                  (sim ltr l /\ sim (union ltr atr) a /\ sim (union ltr btr) b))
-                        (ensures (pre_cond_merge l a b) /\ (sim (abs_merge ltr atr btr) (merge l a b)))
-
-#set-options "--z3rlimit 10000"
-let prop_merge5 ltr l atr a btr b =
-  lemma1 ltr atr; 
-  lemma1 ltr btr;
-  lemma2 ltr atr btr;
-  prop_merge1 ltr l atr a btr b;
-  prop_merge2 ltr l atr a btr b;
-  prop_merge3 ltr l atr a btr b;
-  prop_merge4 ltr l atr a btr b
-*)
+let prop_merge00 l a b opa opb = ()
