ictr.fst
@@ -1,173 +1,212 @@
 module Ictr
+
 open FStar.List.Tot
 
-#set-options "--query_stats"
+val get_id : #op:eqtype -> (nat * op) -> nat
+let get_id (id, _) = id
 
-open Library
+val get_op : #op:eqtype -> (nat * op) -> op
+let get_op (_, op) = op
 
-(** Concrete state of the MRDT*)
+val mem_id : #op:eqtype
+           -> id:nat
+           -> l:list (nat * op)
+           -> Tot (b:bool{(exists op. mem (id,op) l) <==> b=true})
+let rec mem_id n l =
+  match l with
+  |[] -> false
+  |(id,_)::xs -> (n = id) || mem_id n xs
+
+val unique_id : #op:eqtype 
+              -> l:list (nat * op)
+              -> Tot bool
+let rec unique_id l =
+  match l with
+  |[] -> true
+  |(id,_)::xs -> not (mem_id id xs) && unique_id xs
+
+val get_eve : #op:eqtype 
+            -> id:nat 
+            -> l:list (nat * op){unique_id l /\ mem_id id l}
+            -> Tot (s:(nat * op) {get_id s = id /\ mem s l})
+let rec get_eve id l =
+  match l with
+  |(id1, x)::xs -> if id = id1 then (id1, x) else get_eve id xs 
+
+val forallb : #a:eqtype
+            -> f:(a -> bool)
+            -> l:list a
+            -> Tot (b:bool{(forall e. mem e l ==> f e) <==> b = true})
+let rec forallb #a f l = 
+  match l with
+  |[] -> true
+  |hd::tl -> if f hd then forallb f tl else false
+
+val existsb : #a:eqtype
+            -> f:(a -> bool)
+            -> l:list a 
+            -> Tot (b:bool{(exists e. mem e l /\ f e) <==> b = true})
+let rec existsb #a f l =
+  match l with
+  |[] -> false
+  |hd::tl -> if f hd then true else existsb f tl
+
+val sorted : #op:eqtype
+           -> l:list(nat * op){unique_id l} -> bool
+let rec sorted #op l =
+  match l with
+  |[] -> true
+  |x::[] -> true
+  |x::xs -> forallb (fun (e:(nat * op)) -> fst x < fst e) xs && sorted xs
+
+val filter : #a:eqtype
+           -> f:(a -> bool)
+           -> l:list a
+           -> Tot (l1:list a {forall e. mem e l1 <==> mem e l /\ f e})
+let rec filter #a f l = 
+  match l with
+  |[] -> []
+  |hd::tl -> if f hd then hd::(filter f tl) else filter f tl
+
+/////////////////////////////////////////
+
+type op =
+  |Inc
+
+///SEQUENTIAL DATA TYPE IMPLEMENTATION///
+
 type s = nat
 
-
-(** Operations supported by the MRDT*)
-type op = |Add
-          |Rd
-
-
-(** Return value of the operations*)
-type rval = |Val : s -> rval
-            |Bot
-
-
-(** Initial state*)
 let init = 0
 
+val do : s -> (nat * op) -> s
+let do s (_, Inc) = s + 1
 
-let pre_cond_do s1 op = true
-let pre_cond_prop_do tr s1 op = true
+val spec : s1:s -> o1:(nat * op) -> o2:(nat * op) -> s
+let spec s1 o1 o2 =
+  do (do s1 o1) o2
 
-
-(** Concrete DO function*)
-val do : s1:s -> o:(nat * op) -> Tot (s2:(s * rval) {get_op o = Add ==> s2 = (s1 + 1, Bot) /\
-                                                 get_op o = Rd ==> s2 = (s1, Val s1)})
-let do s1 o =
-  match o with
-  |(_,Add) -> (s1 + 1, Bot)
-  |(_,Rd) -> (s1, Val s1)
-
-val sum : l:(list (nat * op))
-        -> Tot (n:nat {n = (List.Tot.length (filter (fun e -> get_op e = Add) l))}) 
-          (decreases %[l])
-let rec sum l =
+val fold : st:s -> l:list (nat * op){unique_id l} -> Tot s (decreases l)
+let rec fold s l =
   match l with
-  |[] -> 0
-  |(_, Add)::xs -> sum xs + 1
-  |(_, Rd)::xs -> sum xs
+  |[] -> s
+  |x::xs -> fold (do s x) xs
+
+////////////MRDT IMPLEMENTATION////////////
+
+type s' = nat
+
+val init' : nat
+let init' = 0
+
+let pre_cond_do' s o = true
+
+val do' : st:s' -> (nat * op) -> r:s'
+let do' s' (_, Inc) = s' + 1
+
+val fold' : st:s' -> l:list (nat * op){unique_id l} -> Tot (st':s' {(st' >= st) /\ (st' = st + length l)})
+            (decreases l)
+let rec fold' s l =
+  match l with
+  |[] -> s
+  |x::xs -> fold' (do' s x) xs
+
+val pre_cond_merge' : l:s' -> a:s' -> b:s' -> bool
+let pre_cond_merge' l a b = a >= l && b >= l
+
+val merge' : l:s' 
+           -> a:s'
+           -> b:s'
+           -> Pure s'
+             (requires pre_cond_merge' l a b)
+             (ensures (fun r -> r = a + b - l))
+let merge' l a b =
+  a + b - l
+
+////////////////////////////////////////////
+
+val eq : st:s -> st':s' -> bool
+let eq s s' = s = s'
+
+val eq_m : a:s' -> b:s' -> bool
+let eq_m a b = a = b
+
+val prop_init : unit -> Lemma (ensures (eq init init'))
+let prop_init () = ()
+
+val prop_equivalence : a:s' -> b:s' -> o:(nat * op)
+                     -> Lemma (requires (eq_m a b /\ pre_cond_do' a o /\ pre_cond_do' b o))
+                             (ensures (eq_m (do' a o) (do' b o)))
+let prop_equivalence a b o = ()
+
+val prop_do : st:s -> st':s' -> o:(nat * op)
+            -> Lemma (requires (eq st st'))
+                    (ensures (eq (do st o) (do' st' o)))
+let prop_do s s' op = ()
+
+val inverse : s:s'{s > 0} -> o:(nat * op) -> r:s'{s = do' r o}
+let inverse a o = a - 1
+
+val append : l1:list(nat * op) -> l2:list(nat * op)
+           -> Pure (list (nat * op))
+                  (requires (forall e. mem e l1 ==> not (mem_id (get_id e) l2)) /\
+                            unique_id l1 /\ unique_id l2)
+                  (ensures (fun r -> (forall e. mem e r <==> mem e l1 \/ mem e l2) /\ unique_id r))
+                  (decreases %[l1;l2])
+let rec append l1 l2 =
+  match l1, l2 with
+  |[],[] -> []
+  |x::xs,_ -> x::(append xs l2)
+  |[],x::xs -> x::(append [] xs)
+
+val prop_merge1 : l:s' -> a:s' -> b:s' 
+                -> atr:list(nat * op) -> o1:(nat * op) 
+                -> btr:list(nat * op) -> o2:(nat * op) 
+                -> Lemma (requires (unique_id atr /\ unique_id btr /\ get_id o1 <> get_id o2 /\
+                                  (forall e. mem e atr ==> not (mem_id (get_id e) btr)) /\
+                                  not (mem_id (get_id o1) atr) /\ not (mem_id (get_id o1) btr) /\
+                                  not (mem_id (get_id o2) atr) /\ not (mem_id (get_id o2) btr) /\
+                                  a = fold' l (append atr [o1]) /\ b = fold' l (append btr [o2])))
+                        (ensures (let merge_prefix = (merge' l (inverse a o1) (inverse b o2)) in 
+                                      ((merge' l a b) = (merge' merge_prefix (do' merge_prefix o1) (do' merge_prefix o2)))))
+let prop_merge1 l a b atr_p o1 btr_p o2 = ()
+
+val prop_merge2 : l:s' -> a:s' -> b:s' -> op1:(nat * op) -> op2:(nat * op)
+                -> Lemma (requires (a = do' l op1 /\ b = do' l op2 /\ get_id op1 <> get_id op2))
+                        (ensures (pre_cond_merge' l a b) /\
+                                 (forall sl. eq sl l ==> (eq (spec sl op1 op2) (merge' l a b))))
+let prop_merge2 l a b opa opb = ()
+
+(*)val prop_merge3 : l:s' -> a:s' -> atr:list(nat * op) -> o1:(nat * op)
+                -> Lemma (requires (unique_id atr /\ (forall e. mem e atr ==> get_id o1 <> get_id e)) /\
+                                  (a = fold' l (append atr [o1])))
+                        (ensures (merge' l a l) = (merge' l (inverse a o1) (do' l o1) ))
+let prop_merge3 l a atr o1 = ()*)
+
+val prop_merge4 : l:s' -> a:s' -> op1:(nat * op)
+                -> Lemma (requires (a = do' l op1))
+                        (ensures (pre_cond_merge' l a l) /\
+                                 (forall sl. eq sl l ==> (eq (do sl op1) (merge' l a l))))
+let prop_merge4 l a op1 = ()
+
+val idempotence : a:s'
+                -> Lemma (ensures (a = (merge' a a a)))
+let idempotence a = ()
+
+val commutativity : l:s' 
+                  -> a:s'
+                  -> b:s'
+                  -> Lemma (requires (exists atr btr. a = fold' l atr /\ b = fold' l btr))
+                          (ensures (merge' l b a = merge' l a b))
+let commutativity l a b = ()
+
+val associativity : l:s'
+                  -> a:s'
+                  -> b:s'
+                  -> c:s'
+                  -> Lemma (requires (exists atr btr ctr. a = fold' l atr /\ b = fold' l btr /\ c = fold' l ctr))
+                          (ensures (merge' l a (merge' l b c) = merge' l (merge' l a b) c))
+let associativity l a b c = ()
 
 
-(** Specification of the MRDT*)
-val spec : o:(nat * op) -> tr:ae op -> rval
-let spec o tr =
-  match o with
-  |(_, Add) -> Bot
-  |(_, Rd) -> Val (sum tr.l)
-
-
-(** Simulation relation*)
-val sim : tr:ae op
-        -> s1:s
-        -> Tot (b:bool {b = true <==> (s1 = sum tr.l)})
-let sim tr s1 = (s1 = sum tr.l)
-
-
-(** Proof of no. of Add operations seen by branch A = no. of Add ops seen by LCA + 
-                                                      no. of Add ops seen by branch A which are not seen by LCA
-    This is needed to show that the concrete state of a >= concrete state of lca.
-    The result of the 3-way merge (a + b - l) is a natural number. 
-    Only with this additional lemma, the merge function will type check. *)
-val sum_union : l_l:list(nat * op) {unique_id l_l}
-              -> a_l:list(nat * op) {unique_id a_l}
-              -> Lemma (requires (forall e. mem e l_l ==> not (mem_id (get_id e) a_l)))
-                      (ensures (sum (union1 l_l a_l) = sum l_l + sum a_l))
-let rec sum_union l_l a_l =
-  match l_l, a_l with
-  |[],[] -> ()
-  |x::xs,_ -> sum_union xs a_l
-  |[],_ -> ()
-
-let pre_cond_merge l a b = a >= l && b >= l
-
-let pre_cond_prop_merge ltr l atr a btr b = true
-
-
-(** Concrete THREE_WAY MERGE function*)
-val merge : l:s -> a:s -> b:s
-          -> Pure s (requires pre_cond_merge l a b)
-                   (ensures (fun r -> r = a + b - l))
-let merge l a b = a + b - l
-
-
-val sum_absmerge : l_l:list(nat * op) {unique_id l_l}
-                 -> a_l:list(nat * op) {unique_id a_l}
-                 -> b_l:list(nat * op) {unique_id b_l}
-                 -> Lemma (requires (forall e. mem e l_l ==> not (mem_id (get_id e) a_l)) /\
-                                   (forall e. mem e a_l ==> not (mem_id (get_id e) b_l)) /\
-                                   (forall e. mem e l_l ==> not (mem_id (get_id e) b_l)))
-                         (ensures (forall e. mem e (abs_merge1 l_l a_l b_l) <==> mem e l_l \/ mem e a_l \/ mem e b_l) /\
-                                  (sum (abs_merge1 l_l a_l b_l) = sum a_l + sum b_l + sum l_l))
-                         (decreases %[l_l;a_l;b_l])
-#set-options "--z3rlimit 1000"
-let rec sum_absmerge l_l a_l b_l =
-  match l_l,a_l,b_l with
-  |[],[],[] -> ()
-  |x::xs,_,_ -> sum_absmerge xs a_l b_l
-  |[],x::xs,_ -> sum_absmerge [] xs b_l
-  |[],[],_ -> ()
-
-
-(** Proof of operations*)
-val prop_do : tr:ae op
-            -> st:s
-            -> op:(nat * op)
-            -> Lemma (requires (sim tr st) /\ (not (mem_id (get_id op) tr.l)) /\
-                              (forall e. mem e tr.l ==> get_id e < get_id op) /\ get_id op > 0)
-                    (ensures (sim (abs_do tr op) (get_st (do st op))))
-let prop_do tr st op = ()
-
-
-(** Proof of three-way merge*)
-val prop_merge : ltr:ae op
-               -> l:s
-               -> atr:ae op
-               -> a:s
-               -> btr:ae op
-               -> b:s
-               -> Lemma (requires (forall e. mem e ltr.l ==> not (mem_id (get_id e) atr.l)) /\
-                                 (forall e. mem e atr.l ==> not (mem_id (get_id e) btr.l)) /\
-                                 (forall e. mem e ltr.l ==> not (mem_id (get_id e) btr.l)) /\
-                                 (sim ltr l /\ sim (union ltr atr) a /\ sim (union ltr btr) b))
-                       (ensures (pre_cond_merge l a b) /\ (sim (abs_merge ltr atr btr) (merge l a b)))
-#set-options "--z3rlimit 1000"
-let prop_merge ltr l atr a btr b = 
-  sum_union ltr.l atr.l; assert (a >= l);
-  sum_union ltr.l btr.l; assert (b >= l);
-  sum_absmerge ltr.l atr.l btr.l
-
-
-
-(** Proof of implementation satisfying the specification*)
-val prop_spec : tr:ae op
-              -> st:s
-              -> op:(nat * op)
-              -> Lemma (requires (sim tr st) /\ (not (mem_id (get_id op) tr.l)) /\
-                                (forall e. mem e tr.l ==> get_id e < get_id op) /\ get_id op > 0)
-                      (ensures (get_rval (do st op) = spec op tr))
-let prop_spec tr st op = ()
-
-
-(** Proof of convergence*)
-val convergence : tr:ae op
-                -> a:s
-                -> b:s
-                -> Lemma (requires (sim tr a /\ sim tr b))
-                        (ensures a = b)
-let convergence tr a b = ()
-
-
-(** ictr is an instance of the MRDT type class satisfying the conditions*)
-instance ictr : mrdt s op rval = {
-  Library.init = init;
-  Library.spec = spec;
-  Library.sim = sim;
-  Library.pre_cond_do = pre_cond_do;
-  Library.pre_cond_prop_do = pre_cond_prop_do;
-  Library.pre_cond_merge = pre_cond_merge;
-  Library.pre_cond_prop_merge = pre_cond_prop_merge;
-  Library.do = do;
-  Library.merge = merge;
-  Library.prop_do = prop_do;
-  Library.prop_merge = prop_merge;
-  Library.prop_spec = prop_spec;
-  Library.convergence = convergence
-}
 
