nn_ctr.fst
@@ -1,344 +1,286 @@
 module Nn_ctr
+
 open FStar.List.Tot
 
-#set-options "--query_stats"
+val get_id : #op:eqtype -> (nat * op) -> nat
+let get_id (id, _) = id
 
-open Library
+val get_op : #op:eqtype -> (nat * op) -> op
+let get_op (_, op) = op
 
-type s = n:nat {n >= 0}
+val mem_id : #op:eqtype
+           -> id:nat
+           -> l:list (nat * op)
+           -> Tot (b:bool{(exists op. mem (id,op) l) <==> b=true})
+let rec mem_id n l =
+  match l with
+  |[] -> false
+  |(id,_)::xs -> (n = id) || mem_id n xs
 
-val init : s
-let init = 0 
+val unique_id : #op:eqtype 
+              -> l:list (nat * op)
+              -> Tot bool
+let rec unique_id l =
+  match l with
+  |[] -> true
+  |(id,_)::xs -> not (mem_id id xs) && unique_id xs
 
-type rval = |Val : s -> rval
-            |Bot
+val get_eve : #op:eqtype 
+            -> id:nat 
+            -> l:list (nat * op){unique_id l /\ mem_id id l}
+            -> Tot (s:(nat * op) {get_id s = id /\ mem s l})
+let rec get_eve id l =
+  match l with
+  |(id1, x)::xs -> if id = id1 then (id1, x) else get_eve id xs 
+
+val forallb : #a:eqtype
+            -> f:(a -> bool)
+            -> l:list a
+            -> Tot (b:bool{(forall e. mem e l ==> f e) <==> b = true})
+let rec forallb #a f l = 
+  match l with
+  |[] -> true
+  |hd::tl -> if f hd then forallb f tl else false
+
+val existsb : #a:eqtype
+            -> f:(a -> bool)
+            -> l:list a 
+            -> Tot (b:bool{(exists e. mem e l /\ f e) <==> b = true})
+let rec existsb #a f l =
+  match l with
+  |[] -> false
+  |hd::tl -> if f hd then true else existsb f tl
+
+val sorted : #op:eqtype
+           -> l:list(nat * op){unique_id l} -> bool
+let rec sorted #op l =
+  match l with
+  |[] -> true
+  |x::[] -> true
+  |x::xs -> forallb (fun (e:(nat * op)) -> fst x < fst e) xs && sorted xs
+
+val filter : #a:eqtype
+           -> f:(a -> bool)
+           -> l:list a
+           -> Tot (l1:list a {forall e. mem e l1 <==> mem e l /\ f e})
+let rec filter #a f l = 
+  match l with
+  |[] -> []
+  |hd::tl -> if f hd then hd::(filter f tl) else filter f tl
+
+/////////////////////////////////////////
 
 type op =
-  |Inc                   //Increment 
-  |Dec : option nat -> op //Decrement op contains the id of the increment op if it matched with it.
-  |Rd                    //Read
+  |Inc
+  |Dec
 
-let pre_cond_do s1 op = true
+///SEQUENTIAL DATA TYPE IMPLEMENTATION///
 
-val do : s1:s
-       -> op:(nat * op)
-       -> Pure (s * rval)
-         (requires pre_cond_do s1 op)
-         (ensures (fun r -> (Inc? (get_op op) ==> r = (s1 + 1, Bot)) /\
-                         (Dec? (get_op op) /\ s1 > 0 ==> r = (s1 - 1, Bot)) /\
-                         (Dec? (get_op op) /\ s1 = 0 ==> r = (s1, Bot)) /\
-                         (Rd? (get_op op) ==> r = (s1, Val s1))))
-let do s1 op1 =
-  match op1 with
-  |(id, Inc) -> (s1 + 1, Bot)
-  |(id, Dec x) -> ((if s1 > 0 then s1 - 1 else s1), Bot)
-  |(id, Rd) -> (s1, Val s1)
+type s = nat
 
-val return : o:(nat * op){Dec? (get_op o)} -> option nat
-let return (_, Dec x) = x
+let init = 0
 
-(** Returns true if 'd' matches with 'i' in tr.l*)
-val matched : i:(nat * op) 
-            -> d:(nat * op)
-            -> tr:ae op
-            -> Pure bool (requires (get_id i <> get_id d))
-                        (ensures (fun b -> (Inc? (get_op i) /\ Dec? (get_op d) /\ mem i tr.l /\ mem d tr.l /\ 
-                                        (return d) = Some (get_id i) /\ (tr.vis i d)) <==> (b = true)))
-let matched i d tr = 
-  (Inc? (get_op i) && Dec? (get_op d)) && (mem i tr.l && mem d tr.l) && (return d) = Some (get_id i) && (tr.vis i d)
+val do : s1:s -> o:(nat * op) -> s2:s{(get_op o = Inc ==> s2 = s1 + 1) /\
+                                  (get_op o = Dec /\ s1 > 0 ==> s2 = s1 - 1) /\
+                                  (get_op o = Dec /\ s1 = 0 ==> s2 = s1)}
+let do s op =
+    match op with
+    |(_,Inc) -> s + 1
+    |(_,Dec) -> if s > 0 then s - 1 else s
 
-val filter_uni : f:((nat * op) -> bool)
-               -> l:list (nat * op) 
-               -> Lemma (requires (unique_id l))
-                       (ensures (unique_id (filter f l)))
-                   [SMTPat (filter f l)]
-let rec filter_uni f l =
+val spec : s1:s -> o1:(nat * op) -> o2:(nat * op) -> s
+let spec s1 o1 o2 =
+    match o1, o2 with
+    |(_,Inc), (_,Dec) -> do (do s1 o2) o1
+    |(_,Dec), (_,Dec) -> do s1 o1
+    |_ -> do (do s1 o1) o2
+
+val fold : st:s -> l:list (nat * op){unique_id l} -> Tot s (decreases l)
+let rec fold s l =
   match l with
-  |[] -> ()
-  |x::xs -> filter_uni f xs
+  |[] -> s
+  |x::xs -> fold (do s x) xs
 
-(** Returns the list of decrement ops that matches 'i' *)
-val dec_match_inc : tr:ae op 
-                  -> i:(nat * op)
-                  -> l:list(nat * op){(forall e. mem e l <==> mem e tr.l /\ Dec? (get_op e) /\ get_id i <> get_id e /\ 
-                                    tr.vis i e /\ matched i e tr) /\ unique_id l /\ 
-                                    ((exists d. mem d tr.l /\ get_id i <> get_id d /\ matched i d tr) <==> (length l > 0)) /\
-                                    (length l > 0 <==> l <> [])}
-let dec_match_inc tr i =
-  filter (fun d -> get_id i <> get_id d && matched i d tr) tr.l
+////////////MRDT IMPLEMENTATION////////////
 
-(** For each increment op there is atmost one matching decrement op.
-    If a decrement operation returns an id, then there should be a matching increment op with that id in tr*)
-assume val axiom : tr:ae op
-                 -> Lemma (ensures (forall i. mem i tr.l /\ Inc? (get_op i) ==> length (dec_match_inc tr i) <= 1) /\
-                                  (forall d id. mem d tr.l /\ Dec? (get_op d) /\ return d = Some id ==> 
-                                    (exists i. mem i tr.l /\ Inc? (get_op i) /\ get_id i <> get_id d /\ tr.vis i d /\ get_id i = id)))
+type s' = n:(nat * nat){fst n >= snd n}
 
-(** Returns the list of increment ops matched with decrement op*)
-val match_inc : tr:ae op
-              -> l:list(nat * op){(forall e. mem e l <==> mem e tr.l /\ Inc? (get_op e) /\ 
-                         (exists d. mem d tr.l /\ Dec? (get_op d) /\ get_id e <> get_id d /\ matched e d tr)) /\ unique_id l}
-let match_inc tr =
-  filter (fun i -> mem i tr.l && Inc? (get_op i) && length (dec_match_inc tr i) > 0) tr.l
+val init' : s'
+let init' = (0, 0)
 
-val remove : ele:(nat * op) 
-           -> a:list(nat * op){unique_id a}
-           -> Tot (b:list(nat * op) {unique_id b /\ (forall e. mem e b <==> mem e a /\ e <> ele) /\
-                                  (mem ele a <==> List.Tot.length b = List.Tot.length a - 1) /\
-                                  (not (mem ele a) <==> List.Tot.length b = List.Tot.length a)})
-let rec remove ele a =
-  match a with
-  |[] -> []
-  |x::xs -> if x = ele then xs else x::(remove ele xs)
+let pre_cond_do' s o = true
 
-(** Returns the list of unmatched increment op*)
-val unmatch_inc : tr:ae op 
-                -> Tot (l:list(nat * op){(forall e. mem e l <==> mem e tr.l /\ Inc? (get_op e) /\ 
-                      (forall d. mem d tr.l /\ Dec? (get_op d) /\ get_id e <> get_id d ==> not (matched e d tr))) /\ unique_id l})
-let unmatch_inc tr =
-  filter (fun i -> Inc? (get_op i) && length (dec_match_inc tr i) = 0) tr.l
+val do' : st:s' -> (nat * op) -> st1:s'{fst st1 >= fst st /\ snd st1 >= snd st}
+let do' s' op =
+    match op with
+    |(_,Inc) -> (fst s' + 1, snd s')
+    |(_,Dec) -> if fst s' > snd s' then (fst s', snd s' + 1) else s'
 
-val lem_length : l:list(nat * op)
-               -> l1:list(nat * op)
-               -> Lemma (requires unique_id l1 /\ unique_id l)
-                       (ensures (forall e. mem e l <==> mem e l1) ==> (length l = length l1))
-                       (decreases %[l;l1])
-let rec lem_length l l1 =
-  match l, l1 with
-  |[],[] -> ()
-  |x::xs,_ -> lem_length xs (remove x l1)
-  |[],_ -> ()
+val tl : l:list(nat * op){l <> []} -> Tot (t:(nat * op){mem t l})
+let rec tl l =
+  match l with
+  |[x] -> x
+  |x::xs -> tl xs
 
-val lem_length1 : a:list (nat * op)
-                -> b:list (nat * op)
-                -> c:list (nat * op)
-                -> Lemma (requires unique_id a /\ unique_id b /\ unique_id c)
-                         (ensures (forall e. mem e a <==> mem e b \/ mem e c) /\
-                                  (forall e. mem e b ==> not (mem e c)) ==> (length a = length b + length c))
-                 (decreases %[a;b;c])
-#set-options "--z3rlimit 1000"
-let rec lem_length1 a b c =
-  match a,b,c with
-  |[],[],[] -> ()
-  |x::xs,_,_ -> lem_length1 xs (remove x b) (remove x c)
-  |[],x::xs,_ -> lem_length1 [] xs (remove x c)
-  |[],[],_ -> ()
+val fold' : st:s' -> l:list (nat * op){unique_id l} -> Tot (st':s' {fst st' >= fst st /\ snd st' >= snd st})
+            (decreases l)
+let rec fold' s l =
+    match l with
+    |[] -> s
+    |x::xs -> fold' (do' s x) xs
 
-#set-options "--initial_fuel 7 --ifuel 7 --initial_ifuel 7 --fuel 7 --z3rlimit 10000"
+val pre_cond_merge' : l:s' -> a:s' -> b:s' -> bool
+let pre_cond_merge' l a b = fst a >= fst l && fst b >= fst l && snd a >= snd l && snd b >= snd l
 
-val spec : o:(nat * op) -> tr:ae op -> rval
-let spec o tr =
+val num_dec_from_lca : l:s' -> a:s'{fst a >= fst l /\ snd a >= snd l} -> Tot nat
+let num_dec_from_lca (il, dl) (ia, da) =
+  if il - dl < da - dl then
+      (* the number of new decrement operations that were performed on the child
+         is greater than the original number of available values in the lca. Then
+         all the values in the lca must have been decremented. *)
+     il - dl
+  else
+      (* Otherwise, the number of lca values decremented is exactly the number of
+         new decrements *)
+     da - dl
+
+val overcount : l:s' -> a:s'{fst a >= fst l /\ snd a >= snd l} -> b:s'{fst b >= fst l /\ snd b >= snd l}
+              -> Tot nat 
+let overcount l a b =
+  let na = num_dec_from_lca l a in
+  let nb = num_dec_from_lca l b in
+  min na nb
+
+(** Concrete THREE_WAY MERGE function*)
+val merge' : l:s' -> a:s' -> b:s'
+             -> Pure s' (requires pre_cond_merge' l a b)
+                   (ensures (fun r -> true))
+let merge' l a b = 
+    let o = overcount l a b in
+    let i = fst a + fst b - fst l in
+    let d = snd a + snd b - snd l in
+    (i, d - o)(* account for the overcount *)
+
+////////////////////////////////////////////
+
+val eq : st:s -> st':s' -> bool
+let eq s s' = s = fst s' - snd s'
+
+val eq_m : a:s' -> b:s' -> bool
+let eq_m a b = fst a - snd a = fst b - snd b
+
+val prop_init : unit -> Lemma (ensures (eq init init'))
+let prop_init () = ()
+
+val prop_equivalence : a:s' -> b:s' -> o:(nat * op)
+                     -> Lemma (requires (eq_m a b /\ pre_cond_do' a o /\ pre_cond_do' b o))
+                             (ensures (eq_m (do' a o) (do' b o)))
+let prop_equivalence a b o = ()
+
+val prop_do : st:s -> st':s' -> o:(nat * op)
+            -> Lemma (requires (eq st st'))
+                    (ensures (eq (do st o) (do' st' o)))
+let prop_do s s' op = ()
+
+val inverse : st:s' -> o:(nat * op) 
+            -> Pure s'
+              (requires (get_op o = Inc ==> fst st > 0 /\ fst st - snd st > 0) /\
+                        (get_op o = Dec ==> snd st > 0))
+              (ensures (fun r -> st = do' r o))
+let inverse a o =
   match o with
-  |(_, Inc) | (_, Dec _) -> Bot
-  |(_, Rd) -> Val (length (unmatch_inc tr))
+  |(_, Inc) -> (fst a - 1, snd a)
+  |(_, Dec) -> (fst a, snd a - 1)
 
-val sim : tr:ae op -> s0:s -> Tot (b:bool{b = true <==> s0 = length (unmatch_inc tr)})
-let sim tr s0 =
-  s0 = length (unmatch_inc tr)
+val append : l1:list(nat * op) -> l2:list(nat * op)
+           -> Pure (list (nat * op))
+                  (requires (forall e. mem e l1 ==> not (mem_id (get_id e) l2)) /\
+                            unique_id l1 /\ unique_id l2)
+                  (ensures (fun r -> (forall e. mem e r <==> mem e l1 \/ mem e l2) /\ unique_id r /\
+                                  (l2 <> [] ==> tl r = tl l2)))
+                  (decreases %[l1;l2])
+let rec append l1 l2 =
+  match l1, l2 with
+  |[],[] -> []
+  |x::xs,_ -> x::(append xs l2)
+  |[],x::xs -> x::(append [] xs)
 
-val convergence : tr:ae op
-                -> a:s
-                -> b:s
-                -> Lemma (requires (sim tr a /\ sim tr b))
-                        (ensures (a = b))
-let convergence tr a b = ()
+val spec' : s1:s' -> o1:(nat * op) -> o2:(nat * op) -> s'
+let spec' s1 o1 o2 =
+    match o1, o2 with
+    |(_,Inc), (_,Dec) -> do' (do' s1 o2) o1
+    |(_,Dec), (_,Dec) -> do' s1 o1
+    |_ -> do' (do' s1 o1) o2
 
-val pre_cond_prop_do : tr:ae op -> st:s -> op:(nat * op)
-                     -> Tot (b:bool {b = true <==> (Dec? (get_op op) /\ st > 0 ==> length (unmatch_inc tr) > 0 /\ 
-                                    (exists i. get_id i <> get_id op /\ matched i op tr)) /\
-                                    (Dec? (get_op op) /\ st <= 0 ==> length (unmatch_inc tr) = 0 /\ return op = None)})
+val prop_merge1 : l:s' -> a:s' -> b:s' 
+                -> atr:list(nat * op) -> o1:(nat * op) 
+                -> btr:list(nat * op) -> o2:(nat * op) 
+                -> Lemma (requires (unique_id atr /\ unique_id btr /\ get_id o1 <> get_id o2 /\
+                                  (forall e. mem e atr ==> not (mem_id (get_id e) btr)) /\
+                                  not (mem_id (get_id o1) atr) /\ not (mem_id (get_id o1) btr) /\
+                                  not (mem_id (get_id o2) atr) /\ not (mem_id (get_id o2) btr) /\
+                                  a = fold' l (append atr [o1]) /\ b = fold' l (append btr [o2]) /\
+                                  (get_op o1 = Inc ==> fst a > 0 /\ fst a - snd a > 0) /\ (get_op o1 = Dec ==> snd a > 0) /\
+                                  (get_op o2 = Inc ==> fst b > 0 /\ fst b - snd b > 0) /\ (get_op o2 = Dec ==> snd b > 0) /\
+                                  (inverse a o1 = fold' l atr /\ inverse b o2 = fold' l btr)))
+                        (ensures (let ia = (inverse a o1) in let ib = (inverse b o2) in
+                                   (let merge_prefix = (merge' l ia ib) in 
+                                      ((merge' l a b) = (merge' merge_prefix (do' merge_prefix o1) (do' merge_prefix o2))))))
 
-let pre_cond_prop_do tr st op =
-  (if (Dec? (get_op op) && st > 0) then (length (unmatch_inc tr) > 0 && (existsb (fun i -> get_id i <> get_id op && matched i op tr) tr.l)) else true) &&
-  (if (Dec? (get_op op) && st <= 0) then (length (unmatch_inc tr) = 0 && return op = None) else true)
+#set-options "--z3rlimit 10000"
+let prop_merge1 l a b atr o1 btr o2 = admit()
 
-val prop_do1 : tr:ae op
-               -> st:s
-               -> op:(nat * op)
-               -> Lemma (requires (sim tr st) /\ not (mem_id (get_id op) tr.l) /\ get_id op > 0 /\
-                                 (forall e. mem e tr.l ==> get_id e < get_id op) /\ Inc? (get_op op) /\
-                                 pre_cond_prop_do tr st op)
-                       (ensures (sim (abs_do tr op) (get_st (do st op))))
-let prop_do1 tr st op =
-  assert (dec_match_inc tr op = []); 
-  assert (forall e. mem e (unmatch_inc (abs_do tr op)) <==> mem e (unmatch_inc tr) \/ e = op);
-  lem_length1 (unmatch_inc (abs_do tr op)) (unmatch_inc tr) [op]
+val prop_merge2 : l:s' -> a:s' -> b:s' -> op1:(nat * op) -> op2:(nat * op)
+                -> Lemma (requires (a = do' l op1 /\ b = do' l op2 /\ get_id op1 <> get_id op2))
+                        (ensures (pre_cond_merge' l a b) /\
+                                 (forall sl. eq sl l ==> (eq (spec sl op1 op2) (merge' l a b))))
+let prop_merge2 l a b opa opb = ()
 
-val prop_do2 : tr:ae op
-               -> st:s
-               -> op:(nat * op)
-               -> Lemma (requires (sim tr st) /\ not (mem_id (get_id op) tr.l) /\ get_id op > 0 /\
-                                 (forall e. mem e tr.l ==> get_id e < get_id op) /\ Dec? (get_op op) /\
-                                 pre_cond_prop_do tr st op)
-                       (ensures (sim (abs_do tr op) (get_st (do st op))))
-let prop_do2 tr st op = ()
+val prop_merge00 : l:s' -> a:s' -> b:s' -> op1:(nat * op) -> op2:(nat * op)
+                -> Lemma (requires (a = do' l op1 /\ b = do' l op2 /\ get_id op1 <> get_id op2 /\
+                                   (exists atr btr. unique_id atr /\ unique_id btr /\
+                                      a = fold' l atr /\ b = fold' l btr)))
+                        (ensures (pre_cond_merge' l a b) /\
+                                 (forall sl. eq sl (merge' l a b) ==> 
+                                    (eq (spec sl op1 op2) (merge' (merge' l a b) 
+                                                                  (do' (merge' l a b) op1)
+                                                                  (do' (merge' l a b) op2)))))
 
-val prop_do3 : tr:ae op
-               -> st:s
-               -> op:(nat * op)
-               -> Lemma (requires (sim tr st) /\ (not (mem_id (get_id op) tr.l)) /\ get_id op > 0 /\
-                                 (forall e. mem e tr.l ==> get_id e < get_id op) /\ Rd? (get_op op))
-                        (ensures (sim (abs_do tr op) (get_st (do st op))))
-let prop_do3 tr st op =
-  assert (forall e. mem e (unmatch_inc tr) <==> mem e (unmatch_inc (abs_do tr op)));
-  lem_length (unmatch_inc tr) (unmatch_inc (abs_do tr op))
+let prop_merge00 l a b opa opb = ()
 
-val prop_do : tr:ae op
-              -> st:s
-              -> op:(nat * op)
-              -> Lemma (requires (sim tr st) /\ not (mem_id (get_id op) tr.l) /\ get_id op > 0 /\
-                                (forall e. mem e tr.l ==> get_id e < get_id op) /\ pre_cond_do tr st /\
-                                pre_cond_prop_do tr st op)
-                      (ensures (sim (abs_do tr op) (get_st (do st op))))
-let prop_do tr st op = 
-  match get_op op with
-  |Inc -> prop_do1 tr st op
-  |Dec _ -> prop_do2 tr st op
-  |Rd -> prop_do3 tr st op
+(*)val prop_merge3 : l:s' -> a:s' -> atr:list(nat * op) -> o1:(nat * op)
+                -> Lemma (requires (unique_id atr /\ not (mem_id (get_id o1) atr) /\
+                                  (a = fold' l (append atr [o1])) /\
+                                  (forall e. mem e (inverse a o1) ==> e = fold' l atr)))
+                        (ensures (forall ia. mem ia (inverse a o1) ==>
+                                    (merge' l a l) = (merge' l ia (do' l o1))))
+let prop_merge3 l a atr o1 = ()*)
 
-val prop_spec : tr:ae op
-              -> st:s
-              -> op:(nat * op)
-              -> Lemma (requires (sim tr st) /\ (not (mem_id (get_id op) tr.l)) /\
-                                (forall e. mem e tr.l ==> get_id e < get_id op) /\ get_id op > 0)
-                      (ensures (get_rval (do st op) = spec op tr))
-let prop_spec tr st op = ()
+val prop_merge4 : l:s' -> a:s' -> op1:(nat * op)
+                -> Lemma (requires (a = do' l op1))
+                        (ensures (pre_cond_merge' l a l) /\
+                                 (forall sl. eq sl l ==> (eq (do sl op1) (merge' l a l))))
+let prop_merge4 l a op1 = ()
 
-val merge : l:s -> a:s -> b:s
-          -> Pure s
-            (requires true)
-            (ensures (fun r -> (((a >= l \/ b >= l) \/ (a + b > l)) <==> r = a + b - l) /\
-                            ((a < l /\ b < l) /\ a + b <= l) ==> r = 0))
-let merge l a b =
-  if ((a >= l || b >= l) || (a + b > l)) then a + b - l else 0
+val idempotence : a:s'
+                -> Lemma (ensures (a = (merge' a a a)))
+let idempotence a = ()
 
-(** Returns the list of unmatched increment ops in l which are matched by decrement ops in a*)
-val match_ltr_atr : l:ae op -> a:ae op
-                  -> Pure (list (nat * op))
-                         (requires (forall e. mem e l.l ==> not (mem_id (get_id e) a.l)))
-                         (ensures (fun r -> (forall e. mem e r <==> mem e (unmatch_inc l) /\ Inc? (get_op e) /\
-                                     (exists d. get_id e <> get_id d && matched e d (union l a))) /\ unique_id r /\
-                                     (length r = length (filter (fun i -> Inc? (get_op i) && 
-                                     (dec_match_inc (union l a) i) <> [] && 
-                                     length (dec_match_inc (union l a) i) > 0) (unmatch_inc l)))))
-let match_ltr_atr l a =
-  filter (fun i -> Inc? (get_op i) && dec_match_inc (union l a) i <> [] && length (dec_match_inc (union l a) i) > 0) (unmatch_inc l)
+val commutativity : l:s' 
+                  -> a:s'
+                  -> b:s'
+                  -> Lemma (requires (exists atr btr. unique_id atr /\ unique_id btr /\ a = fold' l atr /\ b = fold' l btr))
+                          (ensures (merge' l b a = merge' l a b))
+let commutativity l a b = ()
 
-val length_union : l:list(nat * op)
-                 -> a:list(nat * op)
-                 -> la:list(nat * op)
-                 -> Lemma (requires unique_id l /\ unique_id a /\ unique_id la /\
-                                   (forall e. mem e l ==> not (mem_id (get_id e) a)) /\
-                                   (forall e. mem e la ==> mem e l) /\
-                                   (forall e. mem e (union1 l a) <==> ((mem e a \/ mem e l) /\ not (mem e la))))
-                         (ensures (length (union1 l a) = length a + length l - length la))
-                         (decreases %[l;a;la])
-let rec length_union l a la =
-  match l,a,la with
-  |[],[],[] -> ()
-  |x::xs,_,_ -> length_union xs a la
-  |[],x::xs,_ -> length_union l xs la
-  |[],[],_ -> ()
+val associativity : l:s'
+                  -> a:s'
+                  -> b:s'
+                  -> c:s'
+                  -> Lemma (requires (exists atr btr ctr. unique_id atr /\ unique_id btr /\ unique_id ctr /\
+                                     a = fold' l atr /\ b = fold' l btr /\ c = fold' l ctr))
+                          (ensures (merge' l a (merge' l b c) = merge' l (merge' l a b) c))
+let associativity l a b c = ()
 
-val lem_union : l:ae op
-               -> a:ae op
-               -> Lemma (requires (forall e. mem e l.l ==> not (mem_id (get_id e) a.l)))
-                       (ensures (forall e. mem e (unmatch_inc (union l a)) <==> mem e (union1 (unmatch_inc l) (unmatch_inc a))))
-                       (decreases %[l.l;a.l])
-let rec lem_union l a =
-  match l.l,a.l with
-  |[],[] -> ()
-  |x::xs,_ -> lem_union (A l.vis xs) a
-  |[],x::xs -> lem_union l (A a.vis xs)
 
-val unmatch_union : l:ae op
-              -> a:ae op
-              -> Lemma (requires (forall e. mem e l.l ==> not (mem_id (get_id e) a.l)))
-                      (ensures (forall e. mem e (unmatch_inc (union l a)) <==> 
-                                  ((mem e (unmatch_inc a) \/ mem e (unmatch_inc l)) /\ not (mem e (match_ltr_atr l a)))) /\
-                               (length (unmatch_inc (union l a)) = 
-                                  length (unmatch_inc a) + length (unmatch_inc l) - length (match_ltr_atr l a)))
-let unmatch_union l a = 
-  lem_union l a; 
-  lem_length (unmatch_inc (union l a)) (union1 (unmatch_inc l) (unmatch_inc a));
-  length_union (unmatch_inc l) (unmatch_inc a) (match_ltr_atr l a)
 
-val length_absmerge : l:list(nat * op)
-                    -> a:list(nat * op)
-                    -> b:list(nat * op)
-                    -> la:list(nat * op)
-                    -> lb:list(nat * op)
-                    -> Lemma (requires unique_id l /\ unique_id a /\ unique_id la /\ unique_id b /\ unique_id lb /\
-                                     (forall e. mem e l ==> not (mem_id (get_id e) a)) /\
-                                     (forall e. mem e a ==> not (mem_id (get_id e) b)) /\
-                                     (forall e. mem e l ==> not (mem_id (get_id e) b)) /\
-                                     (forall e. mem e la ==> mem e l) /\ (forall e. mem e lb ==> mem e l) /\
-                                     (forall e. mem e la ==> not (mem e lb)) /\
-                      (forall e. mem e (abs_merge1 l a b) <==> ((mem e a \/ mem e b \/ mem e l) /\ not (mem e la) /\ not (mem e lb))))
-                         (ensures (length (abs_merge1 l a b) = length a + length b + length l - length la - length lb))
-                         (decreases %[l;a;b;la;lb])
-let rec length_absmerge l a b la lb =
-  match l,a,b,la,lb with
-  |[],[],[],[],[] -> ()
-  |x::xs,_,_,_,_ -> length_absmerge xs a b la lb
-  |[],x::xs,_,_,_ -> length_absmerge l xs b la lb
-  |[],[],x::xs,_,_ -> length_absmerge l a xs la lb
-  |[],[],[],x::xs,_ -> length_absmerge l a b xs lb
-  |[],[],[],[],x::xs -> length_absmerge l a b la xs
-
-val unmatch_absmerge : l:ae op
-                     -> a:ae op
-                     -> b:ae op
-                     -> Lemma (requires (forall e. mem e l.l ==> not (mem_id (get_id e) a.l)) /\
-                                       (forall e. mem e a.l ==> not (mem_id (get_id e) b.l)) /\
-                                       (forall e. mem e l.l ==> not (mem_id (get_id e) b.l)) /\
-                                       (forall e. mem e (match_ltr_atr l a) ==> not (mem e (match_ltr_atr l b))))
-                             (ensures (forall e. mem e (unmatch_inc (abs_merge l a b)) <==> 
-                             ((mem e (unmatch_inc a) \/ mem e (unmatch_inc b) \/ mem e (unmatch_inc l)) /\
-                               not (mem e (match_ltr_atr l a)) /\ not (mem e (match_ltr_atr l b)))) /\
-                        (length (unmatch_inc (abs_merge l a b)) = 
-                                      length (unmatch_inc a) + length (unmatch_inc b) + length (unmatch_inc l) 
-                                      - length (match_ltr_atr l a) - length (match_ltr_atr l b)))
-let unmatch_absmerge l a b = 
-  lem_union l a; lem_union l b; 
-  lem_length (unmatch_inc (union l a)) (union1 (unmatch_inc l) (unmatch_inc a)); 
-  lem_length (unmatch_inc (union l b)) (union1 (unmatch_inc l) (unmatch_inc b));
-  lem_length (unmatch_inc (abs_merge l a b)) (abs_merge1 (unmatch_inc l) (unmatch_inc a) (unmatch_inc b)); 
-  length_union (unmatch_inc l) (unmatch_inc a) (match_ltr_atr l a);
-  length_union (unmatch_inc l) (unmatch_inc b) (match_ltr_atr l b);
-  length_absmerge (unmatch_inc l) (unmatch_inc a) (unmatch_inc b) (match_ltr_atr l a) (match_ltr_atr l b); ()
-
-let pre_cond_merge l a b = true
-let pre_cond_prop_merge ltr l atr a btr b = true
-
-val prop_merge : ltr:ae op
-               -> l:s
-               -> atr:ae op
-               -> a:s
-               -> btr:ae op
-               -> b:s
-               -> Lemma (requires (forall e. mem e ltr.l ==> not (mem_id (get_id e) atr.l)) /\
-                                 (forall e. mem e atr.l ==> not (mem_id (get_id e) btr.l)) /\
-                                 (forall e. mem e ltr.l ==> not (mem_id (get_id e) btr.l)) /\
-                                 (sim ltr l /\ sim (union ltr atr) a /\ sim (union ltr btr) b))
-                       (ensures (sim (abs_merge ltr atr btr) (merge l a b)))
-let prop_merge ltr l atr a btr b = 
-  unmatch_union ltr atr;
-  unmatch_union ltr btr;
-  unmatch_absmerge ltr atr btr
-
-instance nn_ctr : mrdt s op rval = {
-  Library.init = init;
-  Library.spec = spec;
-  Library.sim = sim;
-  Library.pre_cond_do = pre_cond_do;
-  Library.pre_cond_prop_do = pre_cond_prop_do;
-  Library.pre_cond_merge = pre_cond_merge;
-  Library.pre_cond_prop_merge = pre_cond_prop_merge;
-  Library.do = do;
-  Library.merge = merge;
-  Library.prop_do = prop_do;
-  Library.prop_merge = prop_merge;
-  Library.prop_spec = prop_spec;
-  Library.convergence = convergence
-}
